coq/Util/OptionSetoid.v
@@ -274,3 +274,4 @@ Ltac destruct_opt_r_equiv :=
     | [ |- RelUtil.opt_r _ None None] => reflexivity
     end
   end.
+
